<rdf:RDF
    xmlns:rdf="http://www.w3.org/1999/02/22-rdf-syntax-ns#"
    xmlns:sadlbasemodel="http://sadl.org/sadlbasemodel"
    xmlns:A="http://arcos.rack/ANALYSIS#"
    xmlns:owl="http://www.w3.org/2002/07/owl#"
    xmlns:sadlimplicitmodel="http://sadl.org/sadlimplicitmodel"
    xmlns:builtinfunctions="http://sadl.org/builtinfunctions"
    xmlns:rdfs="http://www.w3.org/2000/01/rdf-schema#"
    xmlns:xsd="http://www.w3.org/2001/XMLSchema#"
  xml:base="http://arcos.rack/ANALYSIS">
  <owl:Ontology rdf:about="">
    <owl:imports rdf:resource="PROV-S"/>
    <owl:imports rdf:resource="http://sadl.org/builtinfunctions"/>
    <owl:imports rdf:resource="http://sadl.org/sadlimplicitmodel"/>
    <owl:imports rdf:resource="http://sadl.org/sadlbasemodel"/>
    <rdfs:comment xml:lang="en">This ontology was created from a SADL file 'ANALYSIS.sadl' and should not be directly edited.</rdfs:comment>
  </owl:Ontology>
  <owl:Class rdf:ID="ANALYSIS_ANNOTATION">
    <rdfs:comment xml:lang="en">A result of the analysis that is linked to some specific part of the system.</rdfs:comment>
    <rdfs:subClassOf rdf:resource="PROV-S#ENTITY"/>
  </owl:Class>
  <owl:Class rdf:ID="ANALYSIS_RESULT">
    <owl:equivalentClass>
      <owl:Class>
        <owl:oneOf rdf:parseType="Collection">
          <A:ANALYSIS_RESULT rdf:ID="Passed"/>
          <A:ANALYSIS_RESULT rdf:ID="Failed"/>
          <A:ANALYSIS_RESULT rdf:ID="Indeterminate"/>
        </owl:oneOf>
      </owl:Class>
    </owl:equivalentClass>
  </owl:Class>
  <owl:Class rdf:ID="ANALYSIS_ANNOTATION_TYPE">
    <rdfs:comment xml:lang="en">An open/extensible set of types of analysis annotations</rdfs:comment>
  </owl:Class>
  <owl:Class rdf:ID="ANALYSIS">
    <rdfs:comment xml:lang="en">ACTIVITY of running some analysis, supposedly creating some ANALYSIS_REPORT</rdfs:comment>
    <rdfs:subClassOf rdf:resource="PROV-S#ACTIVITY"/>
  </owl:Class>
  <owl:Class rdf:ID="ANALYSIS_REPORT">
    <rdfs:comment xml:lang="en">output of an ANALYSIS</rdfs:comment>
    <rdfs:subClassOf rdf:resource="PROV-S#ENTITY"/>
  </owl:Class>
  <owl:ObjectProperty rdf:ID="producedBy">
    <rdfs:subPropertyOf rdf:resource="PROV-S#wasGeneratedBy"/>
    <rdfs:range rdf:resource="PROV-S#ACTIVITY"/>
    <rdfs:domain rdf:resource="#ANALYSIS_REPORT"/>
  </owl:ObjectProperty>
  <owl:ObjectProperty rdf:ID="performedBy">
    <rdfs:subPropertyOf rdf:resource="PROV-S#wasAssociatedWith"/>
    <rdfs:comment xml:lang="en">Entity that is responsible for producing an analysis, could be a person or a tool. </rdfs:comment>
    <rdfs:range rdf:resource="PROV-S#AGENT"/>
    <rdfs:domain rdf:resource="#ANALYSIS"/>
  </owl:ObjectProperty>
  <owl:ObjectProperty rdf:ID="analyzes">
    <rdfs:subPropertyOf rdf:resource="PROV-S#wasDerivedFrom"/>
    <rdfs:comment xml:lang="en">ENTITY(s) under analysis</rdfs:comment>
    <rdfs:range rdf:resource="PROV-S#ENTITY"/>
    <rdfs:domain rdf:resource="#ANALYSIS_REPORT"/>
  </owl:ObjectProperty>
  <owl:ObjectProperty rdf:ID="annotationType">
    <rdfs:comment xml:lang="en">The type of the annotation.</rdfs:comment>
    <rdfs:range rdf:resource="#ANALYSIS_ANNOTATION_TYPE"/>
    <rdfs:domain rdf:resource="#ANALYSIS_ANNOTATION"/>
  </owl:ObjectProperty>
  <owl:ObjectProperty rdf:ID="fromReport">
    <rdfs:comment xml:lang="en">Which analysis report this annotation comes from.</rdfs:comment>
    <rdfs:range rdf:resource="PROV-S#ENTITY"/>
    <rdfs:domain rdf:resource="#ANALYSIS_ANNOTATION"/>
  </owl:ObjectProperty>
  <owl:ObjectProperty rdf:ID="result">
    <rdfs:comment xml:lang="en">one of Passed, Failed, or Indeterminate</rdfs:comment>
    <rdfs:range rdf:resource="#ANALYSIS_RESULT"/>
    <rdfs:domain rdf:resource="#ANALYSIS_REPORT"/>
  </owl:ObjectProperty>
  <owl:DatatypeProperty rdf:ID="description">
    <rdfs:comment xml:lang="en">The content of the annotation.</rdfs:comment>
    <rdfs:range rdf:resource="http://www.w3.org/2001/XMLSchema#string"/>
    <rdfs:domain rdf:resource="#ANALYSIS_ANNOTATION"/>
  </owl:DatatypeProperty>
  <A:ANALYSIS_ANNOTATION_TYPE rdf:ID="POSTCONDITION">
    <rdfs:comment xml:lang="en">A constraint that should hold after of successful operation of this unit of code.</rdfs:comment>
  </A:ANALYSIS_ANNOTATION_TYPE>
  <A:ANALYSIS_ANNOTATION_TYPE rdf:ID="INVARIANT">
    <rdfs:comment xml:lang="en">A constraint on this unit of code or data that is true at any point in the program's execution.</rdfs:comment>
  </A:ANALYSIS_ANNOTATION_TYPE>
  <A:ANALYSIS_ANNOTATION_TYPE rdf:ID="PRECONDITION">
    <rdfs:comment xml:lang="en">A constraint that should hold in advance of successful operation of this unit of code.</rdfs:comment>
  </A:ANALYSIS_ANNOTATION_TYPE>
</rdf:RDF>
