<rdf:RDF
    xmlns:rdf="http://www.w3.org/1999/02/22-rdf-syntax-ns#"
    xmlns:provs="http://arcos.rack/PROV-S#"
    xmlns:builtinfunctions="http://sadl.org/builtinfunctions#"
    xmlns:owl="http://www.w3.org/2002/07/owl#"
    xmlns:Pr="http://arcos.rack/PROCESS#"
    xmlns:sadlimplicitmodel="http://sadl.org/sadlimplicitmodel#"
    xmlns:rdfs="http://www.w3.org/2000/01/rdf-schema#"
    xmlns:sadlbasemodel="http://sadl.org/sadlbasemodel#"
    xmlns:xsd="http://www.w3.org/2001/XMLSchema#"
  xml:base="http://arcos.rack/PROCESS">
  <owl:Ontology rdf:about="">
    <owl:imports rdf:resource="PROV-S"/>
    <owl:imports rdf:resource="http://sadl.org/builtinfunctions"/>
    <owl:imports rdf:resource="http://sadl.org/sadlimplicitmodel"/>
    <owl:imports rdf:resource="http://sadl.org/sadlbasemodel"/>
    <rdfs:comment xml:lang="en">This ontology was created from a SADL file 'PROCESS.sadl' and should not be directly edited.</rdfs:comment>
  </owl:Ontology>
  <owl:Class rdf:ID="OBJECTIVE">
    <rdfs:comment xml:lang="en">An OBJECTIVE identifies tasks from a process for which evidence must be provided to show that the task has been completed. </rdfs:comment>
    <rdfs:subClassOf rdf:resource="PROV-S#ENTITY"/>
  </owl:Class>
  <owl:ObjectProperty rdf:ID="satisfiedBy">
    <rdfs:comment xml:lang="en">An ACTIVITY that demonstrates that the OBJECTIVE has been satisfied.</rdfs:comment>
    <rdfs:range rdf:resource="PROV-S#ACTIVITY"/>
    <rdfs:domain rdf:resource="#OBJECTIVE"/>
  </owl:ObjectProperty>
  <owl:DatatypeProperty rdf:ID="description">
    <rdfs:comment xml:lang="en">Textual description of the OBJECTIVE</rdfs:comment>
    <rdfs:range rdf:resource="http://www.w3.org/2001/XMLSchema#string"/>
    <rdfs:domain rdf:resource="#OBJECTIVE"/>
  </owl:DatatypeProperty>
</rdf:RDF>
