<rdf:RDF
    xmlns:rdf="http://www.w3.org/1999/02/22-rdf-syntax-ns#"
    xmlns:sadlbasemodel="http://sadl.org/sadlbasemodel"
    xmlns:provs="http://arcos.rack/PROV-S#"
    xmlns:owl="http://www.w3.org/2002/07/owl#"
    xmlns:sadlimplicitmodel="http://sadl.org/sadlimplicitmodel"
    xmlns:builtinfunctions="http://sadl.org/builtinfunctions"
    xmlns:rdfs="http://www.w3.org/2000/01/rdf-schema#"
    xmlns:xsd="http://www.w3.org/2001/XMLSchema#"
  xml:base="http://arcos.rack/PROV-S">
  <owl:Ontology rdf:about="">
    <owl:imports rdf:resource="http://sadl.org/builtinfunctions"/>
    <owl:imports rdf:resource="http://sadl.org/sadlimplicitmodel"/>
    <owl:imports rdf:resource="http://sadl.org/sadlbasemodel"/>
    <rdfs:comment xml:lang="en">a basic Implementation of PROV Data Model standard in SADL based on table https://www.w3.org/TR/prov-dm/#relations-at-a-glance</rdfs:comment>
    <rdfs:comment xml:lang="en">This ontology was created from a SADL file 'PROV-S.sadl' and should not be directly edited.</rdfs:comment>
  </owl:Ontology>
  <owl:Class rdf:ID="AGENT">
    <rdfs:comment xml:lang="en">An agent is something that bears some form of responsibility for an activity taking place, for the existence of an entity, or for another agent's activity.</rdfs:comment>
  </owl:Class>
  <owl:Class rdf:ID="ENTITY">
    <rdfs:comment xml:lang="en">An entity is a physical, digital, conceptual, or other kind of thing with some fixed aspects; entities may be real or imaginary.</rdfs:comment>
  </owl:Class>
  <owl:Class rdf:ID="ACTIVITY">
    <rdfs:comment xml:lang="en">An activity is something that occurs over a period of time and acts upon or with entities; it may include consuming, processing, transforming, modifying, relocating, using, or generating entities.</rdfs:comment>
  </owl:Class>
  <owl:ObjectProperty rdf:ID="wasGeneratedBy">
    <rdfs:comment xml:lang="en">Generation is the completion of production of a new entity by an activity. This entity did not exist before generation and becomes available for usage after this generation.</rdfs:comment>
    <rdfs:range rdf:resource="#ACTIVITY"/>
    <rdfs:domain rdf:resource="#ENTITY"/>
  </owl:ObjectProperty>
  <owl:ObjectProperty rdf:ID="wasInformedBy">
    <rdfs:comment xml:lang="en">a Communication, the exchange of some unspecified entity by two activities, one activity using some entity generated by the other.</rdfs:comment>
    <rdfs:range rdf:resource="#ACTIVITY"/>
    <rdfs:domain rdf:resource="#ACTIVITY"/>
  </owl:ObjectProperty>
  <owl:ObjectProperty rdf:ID="wasAttributedTo">
    <rdfs:comment xml:lang="en">Attribution is the ascribing of an entity to an agent. https://www.w3.org/TR/prov-dm/#concept-attribution</rdfs:comment>
    <rdfs:range rdf:resource="#AGENT"/>
    <rdfs:domain rdf:resource="#ENTITY"/>
  </owl:ObjectProperty>
  <owl:ObjectProperty rdf:ID="wasDerivedFrom">
    <rdfs:comment xml:lang="en">A derivation is a transformation of an entity into another, an update of an entity resulting in a new one, or the construction of a new entity based on a pre-existing entity.</rdfs:comment>
    <rdfs:range rdf:resource="#ENTITY"/>
    <rdfs:domain rdf:resource="#ENTITY"/>
  </owl:ObjectProperty>
  <owl:ObjectProperty rdf:ID="uniqueIdentifier">
    <rdfs:domain>
      <owl:Class>
        <owl:unionOf rdf:parseType="Collection">
          <owl:Class rdf:about="#ENTITY"/>
          <owl:Class rdf:about="#AGENT"/>
          <owl:Class rdf:about="#ACTIVITY"/>
        </owl:unionOf>
      </owl:Class>
    </rdfs:domain>
    <rdfs:comment xml:lang="en">uniqueIdentifier is any data item that is used to associate items on when loading into the data store, and must be unique across the entire data set.</rdfs:comment>
    <rdfs:range rdf:resource="http://www.w3.org/2001/XMLSchema#string"/>
    <rdf:type rdf:resource="http://www.w3.org/2002/07/owl#DatatypeProperty"/>
  </owl:ObjectProperty>
  <owl:ObjectProperty rdf:ID="wasAssociatedWith">
    <rdfs:comment xml:lang="en">An activity association is an assignment of responsibility to an agent for an activity, indicating that the agent had a role in the activity. It further allows for a plan to be specified, which is the plan intended by the agent to achieve some goals in the context of this activity.</rdfs:comment>
    <rdfs:range rdf:resource="#AGENT"/>
    <rdfs:domain rdf:resource="#ACTIVITY"/>
  </owl:ObjectProperty>
  <owl:ObjectProperty rdf:ID="actedOnBehalfOf">
    <rdfs:comment xml:lang="en">Delegation is the assignment of authority and responsibility to an agent (by itself or by another agent) to carry out a specific activity as a delegate or representative, while the agent it acts on behalf of retains some responsibility for the outcome of the delegated work.</rdfs:comment>
    <rdfs:range rdf:resource="#AGENT"/>
    <rdfs:domain rdf:resource="#AGENT"/>
  </owl:ObjectProperty>
  <owl:ObjectProperty rdf:ID="used">
    <rdfs:comment xml:lang="en">Usage is the beginning of utilizing an entity by an activity. Before usage, the activity had not begun to utilize this entity and could not have been affected by the entity. (Note: This definition is formulated for a given usage; it is permitted for an activity to have used a same entity multiple times.)</rdfs:comment>
    <rdfs:range rdf:resource="#ENTITY"/>
    <rdfs:domain rdf:resource="#ACTIVITY"/>
  </owl:ObjectProperty>
</rdf:RDF>
