<rdf:RDF
    xmlns:rdf="http://www.w3.org/1999/02/22-rdf-syntax-ns#"
    xmlns:provs="http://arcos.rack/PROV-S#"
    xmlns:builtinfunctions="http://sadl.org/builtinfunctions#"
    xmlns:owl="http://www.w3.org/2002/07/owl#"
    xmlns:sadlimplicitmodel="http://sadl.org/sadlimplicitmodel#"
    xmlns:rdfs="http://www.w3.org/2000/01/rdf-schema#"
    xmlns:sacms="http://arcos.rack/SACM-S#"
    xmlns:sadlbasemodel="http://sadl.org/sadlbasemodel#"
    xmlns:xsd="http://www.w3.org/2001/XMLSchema#"
  xml:base="http://arcos.rack/SACM-S">
  <owl:Ontology rdf:about="">
    <owl:imports rdf:resource="PROV-S"/>
    <owl:imports rdf:resource="http://sadl.org/builtinfunctions"/>
    <owl:imports rdf:resource="http://sadl.org/sadlimplicitmodel"/>
    <owl:imports rdf:resource="http://sadl.org/sadlbasemodel"/>
    <rdfs:comment xml:lang="en">This ontology is based on a sub-set of the Structured Assurance Case Metamodel (SACM, https://omg.org/spec/SACM). This subset is the important elements for constructing the structure of a assurance argument, but does not include all information from the meta-model.</rdfs:comment>
    <rdfs:comment xml:lang="en">This ontology was created from a SADL file 'SACM-S.sadl' and should not be directly edited.</rdfs:comment>
  </owl:Ontology>
  <owl:Class rdf:ID="ASSERTED_CONTEXT">
    <rdfs:comment xml:lang="en">Asserted Context can be used to declare that the artifact cited by an ArtifactReference(s) provides the context for the&#xD;
interpretation and scoping of a Claim or ArgumentReasoning element.</rdfs:comment>
    <rdfs:subClassOf rdf:resource="PROV-S#ENTITY"/>
  </owl:Class>
  <owl:Class rdf:ID="ASSERTED_INFERENCE">
    <rdfs:comment xml:lang="en">Asserted Inference association records the inference that a user declares to exist between one or more Assertion (premise) and&#xD;
another Assertion (conclusion).</rdfs:comment>
    <rdfs:subClassOf rdf:resource="PROV-S#ENTITY"/>
  </owl:Class>
  <owl:Class rdf:ID="ARTIFACT_REFERENCE">
    <rdfs:comment xml:lang="en">Artifact Reference enables the citation of an artifact as information that relates to the structured argument.</rdfs:comment>
    <rdfs:subClassOf rdf:resource="PROV-S#ENTITY"/>
  </owl:Class>
  <owl:Class rdf:ID="ARGUMENT_PACKAGE">
    <rdfs:comment xml:lang="en">Argument Package is the containing element for a structured argument represented using the SACM Argumentation&#xD;
Metamodel.</rdfs:comment>
    <rdfs:subClassOf rdf:resource="PROV-S#ENTITY"/>
  </owl:Class>
  <owl:Class rdf:ID="ARGUMENT_REASONING">
    <rdfs:comment xml:lang="en">Argument Reasoning can be used to provide additional description or explanation of the asserted relationship.</rdfs:comment>
    <rdfs:subClassOf rdf:resource="PROV-S#ENTITY"/>
  </owl:Class>
  <owl:Class rdf:ID="CLAIM">
    <rdfs:comment xml:lang="en">Claims are used to record the propositions of any structured argument contained in an Argument Package.</rdfs:comment>
    <rdfs:subClassOf rdf:resource="PROV-S#ENTITY"/>
  </owl:Class>
  <owl:ObjectProperty rdf:ID="reasoning">
    <rdfs:subPropertyOf rdf:resource="PROV-S#wasDerivedFrom"/>
    <rdfs:range rdf:resource="PROV-S#ENTITY"/>
    <rdfs:domain rdf:resource="#ASSERTED_INFERENCE"/>
  </owl:ObjectProperty>
  <owl:ObjectProperty rdf:ID="target">
    <rdfs:domain>
      <owl:Class>
        <owl:unionOf rdf:parseType="Collection">
          <owl:Class rdf:about="#ASSERTED_CONTEXT"/>
          <owl:Class rdf:about="#ASSERTED_INFERENCE"/>
        </owl:unionOf>
      </owl:Class>
    </rdfs:domain>
    <rdfs:range rdf:resource="PROV-S#ENTITY"/>
    <rdfs:subPropertyOf rdf:resource="PROV-S#wasDerivedFrom"/>
  </owl:ObjectProperty>
  <owl:ObjectProperty rdf:ID="source">
    <rdfs:domain>
      <owl:Class>
        <owl:unionOf rdf:parseType="Collection">
          <owl:Class rdf:about="#ASSERTED_CONTEXT"/>
          <owl:Class rdf:about="#ASSERTED_INFERENCE"/>
        </owl:unionOf>
      </owl:Class>
    </rdfs:domain>
    <rdfs:range rdf:resource="PROV-S#ENTITY"/>
    <rdfs:subPropertyOf rdf:resource="PROV-S#wasDerivedFrom"/>
  </owl:ObjectProperty>
  <owl:ObjectProperty rdf:ID="argumentationElement">
    <rdfs:subPropertyOf rdf:resource="PROV-S#wasDerivedFrom"/>
    <rdfs:range rdf:resource="PROV-S#ENTITY"/>
    <rdfs:domain rdf:resource="#ARGUMENT_PACKAGE"/>
  </owl:ObjectProperty>
</rdf:RDF>
