<rdf:RDF
    xmlns:rdf="http://www.w3.org/1999/02/22-rdf-syntax-ns#"
    xmlns:sw="http://arcos.rack/SOFTWARE#"
    xmlns:sadlbasemodel="http://sadl.org/sadlbasemodel"
    xmlns:j.0="http://arcos.rack/PROV-S#"
    xmlns:provs="http://arcos.rack/PROV-S"
    xmlns:owl="http://www.w3.org/2002/07/owl#"
    xmlns:sadlimplicitmodel="http://sadl.org/sadlimplicitmodel"
    xmlns:builtinfunctions="http://sadl.org/builtinfunctions"
    xmlns:rdfs="http://www.w3.org/2000/01/rdf-schema#"
    xmlns:xsd="http://www.w3.org/2001/XMLSchema#"
  xml:base="http://arcos.rack/SOFTWARE">
  <owl:Ontology rdf:about="">
    <owl:imports rdf:resource="PROV-S"/>
    <owl:imports rdf:resource="http://sadl.org/builtinfunctions"/>
    <owl:imports rdf:resource="http://sadl.org/sadlimplicitmodel"/>
    <owl:imports rdf:resource="http://sadl.org/sadlbasemodel"/>
    <rdfs:comment xml:lang="en">This ontology was created from a SADL file 'SOFTWARE.sadl' and should not be directly edited.</rdfs:comment>
  </owl:Ontology>
  <owl:Class rdf:ID="COMPILE">
    <rdfs:comment xml:lang="en">ACTIVITY of running a a COMPILER to produce EXECUTABLEs or OBJECT_FILEs</rdfs:comment>
    <rdfs:subClassOf rdf:resource="PROV-S#ACTIVITY"/>
  </owl:Class>
  <owl:Class rdf:ID="LIBRARY">
    <rdfs:comment xml:lang="en">shared library</rdfs:comment>
    <rdfs:subClassOf rdf:resource="PROV-S#ENTITY"/>
  </owl:Class>
  <owl:Class rdf:ID="PACKAGE_FILE">
    <rdfs:comment xml:lang="en">a package file, e.g. Reg Hat's .rpm, Debian's .deb, etc.</rdfs:comment>
    <rdfs:subClassOf rdf:resource="PROV-S#ENTITY"/>
  </owl:Class>
  <owl:Class rdf:ID="CODE_GENERATOR">
    <rdfs:comment xml:lang="en">a tool that generates CODE_FILEs as part of a CODE_GEN ACTIVITY</rdfs:comment>
    <rdfs:subClassOf rdf:resource="PROV-S#AGENT"/>
  </owl:Class>
  <owl:Class rdf:ID="CODE_FILE">
    <rdfs:comment xml:lang="en">file that contains code that may be compiled and/or executed</rdfs:comment>
    <rdfs:subClassOf rdf:resource="PROV-S#ENTITY"/>
  </owl:Class>
  <owl:Class rdf:ID="COMPONENT">
    <rdfs:subClassOf>
      <owl:Restriction>
        <owl:cardinality rdf:datatype="http://www.w3.org/2001/XMLSchema#int"
        >1</owl:cardinality>
        <owl:onProperty>
          <owl:ObjectProperty rdf:ID="componentType"/>
        </owl:onProperty>
      </owl:Restriction>
    </rdfs:subClassOf>
    <rdfs:subClassOf rdf:resource="PROV-S#ENTITY"/>
  </owl:Class>
  <owl:Class rdf:ID="LANGUAGE">
    <rdfs:comment xml:lang="en">describes a programming language, possibly identifying some version of its specification</rdfs:comment>
    <rdfs:subClassOf rdf:resource="PROV-S#ENTITY"/>
  </owl:Class>
  <owl:Class rdf:ID="CODE_GEN">
    <rdfs:comment xml:lang="en">ACTIVITY of running a CODE_GENERATOR to create CODE_FILEs</rdfs:comment>
    <rdfs:subClassOf rdf:resource="PROV-S#ACTIVITY"/>
  </owl:Class>
  <owl:Class rdf:ID="OBJECT_FILE">
    <rdfs:comment xml:lang="en">compiled object code, not ready for execution</rdfs:comment>
    <rdfs:subClassOf rdf:resource="PROV-S#ENTITY"/>
  </owl:Class>
  <owl:Class rdf:ID="BUILD">
    <rdfs:comment xml:lang="en">describes a set of ACTIVITYs (e.g. CODE_GEN, COMPILE, ...) that together form some logical building unit</rdfs:comment>
    <rdfs:subClassOf rdf:resource="PROV-S#ACTIVITY"/>
  </owl:Class>
  <owl:Class rdf:ID="COMPONENT_TYPE">
    <rdfs:subClassOf>
      <owl:Restriction>
        <owl:cardinality rdf:datatype="http://www.w3.org/2001/XMLSchema#int"
        >1</owl:cardinality>
        <owl:onProperty>
          <rdf:Description rdf:about="PROV-S#uniqueIdentifier">
            <rdfs:domain rdf:resource="#COMPONENT_TYPE"/>
          </rdf:Description>
        </owl:onProperty>
      </owl:Restriction>
    </rdfs:subClassOf>
    <rdfs:comment xml:lang="en">An open/extensible set of types of software components</rdfs:comment>
  </owl:Class>
  <owl:Class rdf:ID="EXECUTABLE">
    <rdfs:comment xml:lang="en">compiled executable, ready for execution</rdfs:comment>
    <rdfs:subClassOf rdf:resource="PROV-S#ENTITY"/>
  </owl:Class>
  <owl:Class rdf:ID="PACKAGER">
    <rdfs:comment xml:lang="en">a tool that packages some software together as part of a PACKAGE ACTIVITY</rdfs:comment>
    <rdfs:subClassOf rdf:resource="PROV-S#AGENT"/>
  </owl:Class>
  <owl:Class rdf:ID="COMPILER">
    <rdfs:comment xml:lang="en">a tool that compiles CODE_FILEs into ENTITYs such as OBJECT_FILE or EXECUTABLE</rdfs:comment>
    <rdfs:subClassOf rdf:resource="PROV-S#AGENT"/>
  </owl:Class>
  <owl:Class rdf:ID="PACKAGE">
    <rdfs:comment xml:lang="en">ACTIVITY of running a PACKAGER to produce a PACKAGE_FILE</rdfs:comment>
    <rdfs:subClassOf rdf:resource="PROV-S#ACTIVITY"/>
  </owl:Class>
  <owl:Class rdf:ID="CONFIG_FILE">
    <rdfs:comment xml:lang="en">anything that can be considered configuration</rdfs:comment>
    <rdfs:subClassOf rdf:resource="PROV-S#ENTITY"/>
  </owl:Class>
  <owl:Class rdf:ID="CODE_DEVELOPMENT">
    <rdfs:comment xml:lang="en">an ACTIVITY that produces CODE_FILEs</rdfs:comment>
    <rdfs:subClassOf rdf:resource="PROV-S#ACTIVITY"/>
  </owl:Class>
  <owl:ObjectProperty rdf:ID="governedBy">
    <rdfs:subPropertyOf rdf:resource="PROV-S#used"/>
    <rdfs:comment xml:lang="en">ENTITY(s) (e.g. REQUIREMENT) that gave rise to this ACTIVITY</rdfs:comment>
    <rdfs:range rdf:resource="PROV-S#ENTITY"/>
    <rdfs:domain rdf:resource="#CODE_DEVELOPMENT"/>
  </owl:ObjectProperty>
  <owl:ObjectProperty rdf:ID="satisfies">
    <rdfs:subPropertyOf rdf:resource="PROV-S#wasDerivedFrom"/>
    <rdfs:comment xml:lang="en">ENTITY(s) (e.g. REQUIREMENT) that this code file participates in satisfying</rdfs:comment>
    <rdfs:range rdf:resource="PROV-S#ENTITY"/>
    <rdfs:domain rdf:resource="#CODE_FILE"/>
  </owl:ObjectProperty>
  <owl:ObjectProperty rdf:ID="subcomponentOf">
    <rdfs:comment xml:lang="en">A structural sub-component, e.g., a function might be a subcomponent of module.</rdfs:comment>
    <rdfs:range rdf:resource="PROV-S#ENTITY"/>
    <rdfs:domain rdf:resource="#COMPONENT"/>
  </owl:ObjectProperty>
  <owl:ObjectProperty rdf:ID="referenced">
    <rdfs:subPropertyOf rdf:resource="PROV-S#used"/>
    <rdfs:comment xml:lang="en">ENTITY(s) (e.g. REQUIREMENT) that were referenced during this ACTIVITY</rdfs:comment>
    <rdfs:range rdf:resource="PROV-S#ENTITY"/>
    <rdfs:domain rdf:resource="#CODE_DEVELOPMENT"/>
  </owl:ObjectProperty>
  <owl:ObjectProperty rdf:ID="instantiates">
    <rdfs:comment xml:lang="en">What logical component (system) does this physical component (code) instantiate or implement?</rdfs:comment>
    <rdfs:range rdf:resource="PROV-S#ENTITY"/>
    <rdfs:domain rdf:resource="#COMPONENT"/>
  </owl:ObjectProperty>
  <owl:ObjectProperty rdf:ID="controlFlowsToConditionally">
    <rdfs:comment xml:lang="en">Control flows from this component to the target conditionally.</rdfs:comment>
    <rdfs:range rdf:resource="#COMPONENT"/>
    <rdfs:domain rdf:resource="#COMPONENT"/>
  </owl:ObjectProperty>
  <owl:ObjectProperty rdf:ID="definedIn">
    <rdfs:comment xml:lang="en">Defining entity of this code structure. This could be a CODE_FILE, LIBRARY, etc.</rdfs:comment>
    <rdfs:range rdf:resource="PROV-S#ENTITY"/>
    <rdfs:domain rdf:resource="#COMPONENT"/>
  </owl:ObjectProperty>
  <owl:ObjectProperty rdf:ID="language">
    <rdfs:subPropertyOf rdf:resource="PROV-S#wasDerivedFrom"/>
    <rdfs:comment xml:lang="en">programming language(s) of this file</rdfs:comment>
    <rdfs:range rdf:resource="#LANGUAGE"/>
    <rdfs:domain rdf:resource="#CODE_FILE"/>
  </owl:ObjectProperty>
  <owl:ObjectProperty rdf:about="#componentType">
    <rdfs:range rdf:resource="#COMPONENT_TYPE"/>
    <rdfs:domain rdf:resource="#COMPONENT"/>
  </owl:ObjectProperty>
  <owl:ObjectProperty rdf:ID="annotations">
    <rdfs:comment xml:lang="en">Analysis annotations that apply to this component.</rdfs:comment>
    <rdfs:range rdf:resource="PROV-S#ENTITY"/>
    <rdfs:domain rdf:resource="#COMPONENT"/>
  </owl:ObjectProperty>
  <owl:ObjectProperty rdf:ID="step">
    <rdfs:subPropertyOf rdf:resource="PROV-S#wasInformedBy"/>
    <rdfs:comment xml:lang="en">a BUILD may be comprised of any number of sub-ACTIVITY(s)</rdfs:comment>
    <rdfs:range rdf:resource="PROV-S#ACTIVITY"/>
    <rdfs:domain rdf:resource="#BUILD"/>
  </owl:ObjectProperty>
  <owl:ObjectProperty rdf:ID="requirements">
    <rdfs:comment xml:lang="en">Low-level requirements that apply to this component.</rdfs:comment>
    <rdfs:range rdf:resource="PROV-S#ENTITY"/>
    <rdfs:domain rdf:resource="#COMPONENT"/>
  </owl:ObjectProperty>
  <owl:ObjectProperty rdf:ID="createBy">
    <rdfs:domain>
      <owl:Class>
        <owl:unionOf rdf:parseType="Collection">
          <owl:Class rdf:about="#CODE_FILE"/>
          <owl:Class rdf:about="#CONFIG_FILE"/>
          <owl:Class rdf:about="#OBJECT_FILE"/>
          <owl:Class rdf:about="#LIBRARY"/>
          <owl:Class rdf:about="#EXECUTABLE"/>
        </owl:unionOf>
      </owl:Class>
    </rdfs:domain>
    <rdfs:comment xml:lang="en">ACTIVITY(s) that created this file</rdfs:comment>
    <rdfs:range rdf:resource="PROV-S#ACTIVITY"/>
    <rdfs:subPropertyOf rdf:resource="PROV-S#wasGeneratedBy"/>
  </owl:ObjectProperty>
  <owl:ObjectProperty rdf:ID="mentions">
    <rdfs:comment xml:lang="en">A component referenced by this one, e.g., a callee or variable being used.</rdfs:comment>
    <rdfs:range rdf:resource="PROV-S#ENTITY"/>
    <rdfs:domain rdf:resource="#COMPONENT"/>
  </owl:ObjectProperty>
  <owl:ObjectProperty rdf:ID="performedBy">
    <rdfs:comment xml:lang="en">AGENT(s) (e.g. PACKAGER) performing the packaging</rdfs:comment>
    <rdfs:comment xml:lang="en">AGENT(s) (e.g. COMPILER) performing the compilation</rdfs:comment>
    <rdfs:domain>
      <owl:Class>
        <owl:unionOf rdf:parseType="Collection">
          <owl:Class rdf:about="#CODE_GEN"/>
          <owl:Class rdf:about="#COMPILE"/>
          <owl:Class rdf:about="#PACKAGE"/>
        </owl:unionOf>
      </owl:Class>
    </rdfs:domain>
    <rdfs:comment xml:lang="en">AGENT(s) (e.g. CODE_GENERATOR) generating the code</rdfs:comment>
    <rdfs:range rdf:resource="PROV-S#AGENT"/>
    <rdfs:subPropertyOf rdf:resource="PROV-S#wasAssociatedWith"/>
  </owl:ObjectProperty>
  <owl:ObjectProperty rdf:ID="author">
    <rdfs:subPropertyOf rdf:resource="PROV-S#wasAssociatedWith"/>
    <rdfs:comment xml:lang="en">AGENT(s) who participated in this ACTIVITY</rdfs:comment>
    <rdfs:range rdf:resource="PROV-S#AGENT"/>
    <rdfs:domain rdf:resource="#CODE_DEVELOPMENT"/>
  </owl:ObjectProperty>
  <owl:ObjectProperty rdf:ID="controlFlowsToUnconditionally">
    <rdfs:comment xml:lang="en">Control flows from this component to the target unconditionally.</rdfs:comment>
    <rdfs:range rdf:resource="#COMPONENT"/>
    <rdfs:domain rdf:resource="#COMPONENT"/>
  </owl:ObjectProperty>
  <owl:DatatypeProperty rdf:ID="name">
    <rdfs:range rdf:resource="http://www.w3.org/2001/XMLSchema#string"/>
    <rdfs:domain rdf:resource="#COMPONENT"/>
  </owl:DatatypeProperty>
  <owl:DatatypeProperty rdf:ID="valueType">
    <rdfs:comment xml:lang="en">The type of this value, if applicable (e.g. for functions or variables).</rdfs:comment>
    <rdfs:range rdf:resource="http://www.w3.org/2001/XMLSchema#string"/>
    <rdfs:domain rdf:resource="#COMPONENT"/>
  </owl:DatatypeProperty>
  <owl:DatatypeProperty rdf:ID="version">
    <rdfs:comment xml:lang="en">version of the language, where applicable</rdfs:comment>
    <rdfs:range rdf:resource="http://www.w3.org/2001/XMLSchema#string"/>
    <rdfs:domain rdf:resource="#LANGUAGE"/>
  </owl:DatatypeProperty>
  <sw:COMPONENT_TYPE rdf:ID="MODULE">
    <j.0:uniqueIdentifier rdf:datatype="http://www.w3.org/2001/XMLSchema#string"
    >MODULE</j.0:uniqueIdentifier>
    <rdfs:comment xml:lang="en">A collection of related code, usually grouped in a lexical scope.</rdfs:comment>
  </sw:COMPONENT_TYPE>
  <sw:COMPONENT_TYPE rdf:ID="CLASS">
    <j.0:uniqueIdentifier rdf:datatype="http://www.w3.org/2001/XMLSchema#string"
    >CLASS</j.0:uniqueIdentifier>
    <rdfs:comment xml:lang="en">A class in an object-oriented language.</rdfs:comment>
  </sw:COMPONENT_TYPE>
  <sw:COMPONENT_TYPE rdf:ID="CLASS_CONSTRUCTOR">
    <j.0:uniqueIdentifier rdf:datatype="http://www.w3.org/2001/XMLSchema#string"
    >CLASS_CONSTRUCTOR</j.0:uniqueIdentifier>
    <rdfs:comment xml:lang="en">A constructor in an object-oriented language.</rdfs:comment>
  </sw:COMPONENT_TYPE>
  <sw:COMPONENT_TYPE rdf:ID="SOURCE_FUNCTION">
    <j.0:uniqueIdentifier rdf:datatype="http://www.w3.org/2001/XMLSchema#string"
    >SOURCE_FUNCTION</j.0:uniqueIdentifier>
    <rdfs:comment xml:lang="en">A function or procedure declared or defined in source code.</rdfs:comment>
  </sw:COMPONENT_TYPE>
  <sw:COMPONENT_TYPE rdf:ID="BINARY_BASIC_BLOCK">
    <j.0:uniqueIdentifier rdf:datatype="http://www.w3.org/2001/XMLSchema#string"
    >BINARY_BASIC_BLOCK</j.0:uniqueIdentifier>
    <rdfs:comment xml:lang="en">A basic block at the binary level.</rdfs:comment>
  </sw:COMPONENT_TYPE>
  <sw:COMPONENT_TYPE rdf:ID="BINARY_GLOBAL_VARIABLE">
    <j.0:uniqueIdentifier rdf:datatype="http://www.w3.org/2001/XMLSchema#string"
    >BINARY_GLOBAL_VARIABLE</j.0:uniqueIdentifier>
    <rdfs:comment xml:lang="en">A global variable (generally in the .data or .bss sections).</rdfs:comment>
  </sw:COMPONENT_TYPE>
  <sw:COMPONENT_TYPE rdf:ID="CLASS_METHOD">
    <j.0:uniqueIdentifier rdf:datatype="http://www.w3.org/2001/XMLSchema#string"
    >CLASS_METHOD</j.0:uniqueIdentifier>
    <rdfs:comment xml:lang="en">A method attached to a class in an object-oriented language.</rdfs:comment>
  </sw:COMPONENT_TYPE>
  <sw:COMPONENT_TYPE rdf:ID="BINARY_FUNCTION">
    <j.0:uniqueIdentifier rdf:datatype="http://www.w3.org/2001/XMLSchema#string"
    >BINARY_FUNCTION</j.0:uniqueIdentifier>
    <rdfs:comment xml:lang="en">A function in a binary, as defined by the appropriate ABI.</rdfs:comment>
  </sw:COMPONENT_TYPE>
  <sw:COMPONENT_TYPE rdf:ID="SOURCE_GLOBAL_VARIABLE">
    <j.0:uniqueIdentifier rdf:datatype="http://www.w3.org/2001/XMLSchema#string"
    >SOURCE_GLOBAL_VARIABLE</j.0:uniqueIdentifier>
    <rdfs:comment xml:lang="en">A global variable declared or defined in source code.</rdfs:comment>
  </sw:COMPONENT_TYPE>
  <sw:COMPONENT_TYPE rdf:ID="NAMESPACE">
    <j.0:uniqueIdentifier rdf:datatype="http://www.w3.org/2001/XMLSchema#string"
    >NAMESPACE</j.0:uniqueIdentifier>
    <rdfs:comment xml:lang="en">A collection of related code, usually grouped in a lexical scope.</rdfs:comment>
  </sw:COMPONENT_TYPE>
  <sw:COMPONENT_TYPE rdf:ID="CLASS_MEMBER_VARIABLE">
    <j.0:uniqueIdentifier rdf:datatype="http://www.w3.org/2001/XMLSchema#string"
    >CLASS_MEMBER_VARIABLE</j.0:uniqueIdentifier>
    <rdfs:comment xml:lang="en">A variable attached to the instances of a class in an object-oriented language.</rdfs:comment>
  </sw:COMPONENT_TYPE>
</rdf:RDF>
