<rdf:RDF
    xmlns:rdf="http://www.w3.org/1999/02/22-rdf-syntax-ns#"
    xmlns:sadlbasemodel="http://sadl.org/sadlbasemodel"
    xmlns:sys="http://arcos.rack/SYSTEM#"
    xmlns:owl="http://www.w3.org/2002/07/owl#"
    xmlns:sadlimplicitmodel="http://sadl.org/sadlimplicitmodel"
    xmlns:builtinfunctions="http://sadl.org/builtinfunctions"
    xmlns:rdfs="http://www.w3.org/2000/01/rdf-schema#"
    xmlns:xsd="http://www.w3.org/2001/XMLSchema#"
  xml:base="http://arcos.rack/SYSTEM">
  <owl:Ontology rdf:about="">
    <owl:imports rdf:resource="PROV-S"/>
    <owl:imports rdf:resource="http://sadl.org/builtinfunctions"/>
    <owl:imports rdf:resource="http://sadl.org/sadlimplicitmodel"/>
    <owl:imports rdf:resource="http://sadl.org/sadlbasemodel"/>
    <rdfs:comment xml:lang="en">This ontology was created from a SADL file 'SYSTEM.sadl' and should not be directly edited.</rdfs:comment>
  </owl:Ontology>
  <owl:Class rdf:ID="SYSTEM_DEVELOPMENT">
    <rdfs:comment xml:lang="en">ACTIVITY relating to the creation of one or more some SYSTEMs</rdfs:comment>
    <rdfs:subClassOf rdf:resource="PROV-S#ACTIVITY"/>
  </owl:Class>
  <owl:Class rdf:ID="SYSTEM">
    <rdfs:comment xml:lang="en">SYSTEMs classify logical parts of the whole system being developed</rdfs:comment>
    <rdfs:subClassOf rdf:resource="PROV-S#ENTITY"/>
  </owl:Class>
  <owl:Class rdf:ID="INTERFACE">
    <rdfs:comment xml:lang="en">INTERFACEs describe directed connections between an ENTITY (e.g. SYSTEM) providing what another ENTITY (e.g. SYSTEM) requires</rdfs:comment>
    <rdfs:subClassOf rdf:resource="PROV-S#ENTITY"/>
  </owl:Class>
  <owl:ObjectProperty rdf:ID="provides">
    <rdfs:subPropertyOf rdf:resource="PROV-S#wasDerivedFrom"/>
    <rdfs:comment xml:lang="en">list of entities that this SYSTEM provides to others</rdfs:comment>
    <rdfs:range rdf:resource="PROV-S#ENTITY"/>
    <rdfs:domain rdf:resource="#SYSTEM"/>
  </owl:ObjectProperty>
  <owl:ObjectProperty rdf:ID="partOf">
    <rdfs:subPropertyOf rdf:resource="PROV-S#wasDerivedFrom"/>
    <rdfs:comment xml:lang="en">used to define a relationship to a higher level system</rdfs:comment>
    <rdfs:range rdf:resource="PROV-S#ENTITY"/>
    <rdfs:domain rdf:resource="#SYSTEM"/>
  </owl:ObjectProperty>
  <owl:ObjectProperty rdf:ID="source">
    <rdfs:subPropertyOf rdf:resource="PROV-S#wasDerivedFrom"/>
    <owl:inverseOf rdf:resource="#provides"/>
    <rdfs:comment xml:lang="en">ENTITY (e.g. SYSTEM) that provides what the INTERFACE offers</rdfs:comment>
    <rdfs:range rdf:resource="PROV-S#ENTITY"/>
    <rdfs:domain rdf:resource="#INTERFACE"/>
  </owl:ObjectProperty>
  <owl:ObjectProperty rdf:ID="producedBy">
    <rdfs:subPropertyOf rdf:resource="PROV-S#wasGeneratedBy"/>
    <rdfs:comment xml:lang="en">trace to ACTIVITYs participating in developing this SYSTEM</rdfs:comment>
    <rdfs:range rdf:resource="PROV-S#ACTIVITY"/>
    <rdfs:domain rdf:resource="#SYSTEM"/>
  </owl:ObjectProperty>
  <owl:ObjectProperty rdf:ID="requires">
    <rdfs:subPropertyOf rdf:resource="PROV-S#wasDerivedFrom"/>
    <rdfs:comment xml:lang="en">list of entities that this SYSTEM requires from others</rdfs:comment>
    <rdfs:range rdf:resource="PROV-S#ENTITY"/>
    <rdfs:domain rdf:resource="#SYSTEM"/>
  </owl:ObjectProperty>
  <owl:ObjectProperty rdf:ID="developedBy">
    <rdfs:comment xml:lang="en">Organization that is responsible for producing a system</rdfs:comment>
    <rdfs:range rdf:resource="PROV-S#AGENT"/>
    <rdfs:domain rdf:resource="#SYSTEM_DEVELOPMENT"/>
  </owl:ObjectProperty>
  <owl:ObjectProperty rdf:ID="identifiedBy">
    <rdfs:subPropertyOf rdf:resource="PROV-S#wasGeneratedBy"/>
    <rdfs:comment xml:lang="en">ACTIVITY out of which this INTERFACE was identified</rdfs:comment>
    <rdfs:range rdf:resource="PROV-S#ACTIVITY"/>
    <rdfs:domain rdf:resource="#INTERFACE"/>
  </owl:ObjectProperty>
  <owl:ObjectProperty rdf:ID="destination">
    <rdfs:subPropertyOf rdf:resource="PROV-S#wasDerivedFrom"/>
    <owl:inverseOf rdf:resource="#requires"/>
    <rdfs:comment xml:lang="en">ENTITY (e.g. SYSTEM) that requires what the INTERFACE offers</rdfs:comment>
    <rdfs:range rdf:resource="PROV-S#ENTITY"/>
    <rdfs:domain rdf:resource="#INTERFACE"/>
  </owl:ObjectProperty>
</rdf:RDF>
