<rdf:RDF
    xmlns:rdf="http://www.w3.org/1999/02/22-rdf-syntax-ns#"
    xmlns:BoeingModel="http://arcos.AH-64D/Boeing#"
    xmlns:builtinfunctions="http://sadl.org/builtinfunctions#"
    xmlns:owl="http://www.w3.org/2002/07/owl#"
    xmlns:sadlimplicitmodel="http://sadl.org/sadlimplicitmodel#"
    xmlns:rdfs="http://www.w3.org/2000/01/rdf-schema#"
    xmlns:sadlbasemodel="http://sadl.org/sadlbasemodel#"
    xmlns:xsd="http://www.w3.org/2001/XMLSchema#"
  xml:base="http://arcos.AH-64D/Boeing">
  <owl:Ontology rdf:about="">
    <owl:imports rdf:resource="http://arcos.rack/TESTING"/>
    <owl:imports rdf:resource="http://arcos.rack/REQUIREMENTS"/>
    <owl:imports rdf:resource="http://sadl.org/builtinfunctions"/>
    <owl:imports rdf:resource="http://sadl.org/sadlimplicitmodel"/>
    <owl:imports rdf:resource="http://sadl.org/sadlbasemodel"/>
    <rdfs:comment xml:lang="en">This ontology was created from a SADL file 'Boeing-Ontology.sadl' and should not be directly edited.</rdfs:comment>
  </owl:Ontology>
  <owl:Class rdf:ID="SubDD_Req">
    <rdfs:subClassOf>
      <owl:Restriction>
        <owl:allValuesFrom>
          <owl:Class rdf:ID="SRS_Req"/>
        </owl:allValuesFrom>
        <owl:onProperty rdf:resource="http://arcos.rack/REQUIREMENTS#satisfies"/>
      </owl:Restriction>
    </rdfs:subClassOf>
    <rdfs:comment xml:lang="en">A Requirement identified in the Subsystem Design Document</rdfs:comment>
    <rdfs:subClassOf rdf:resource="http://arcos.rack/REQUIREMENTS#REQUIREMENT"/>
  </owl:Class>
  <owl:Class rdf:about="#SRS_Req">
    <rdfs:comment xml:lang="en">A Requirement identified in the Software Requirements Specification</rdfs:comment>
    <rdfs:subClassOf rdf:resource="http://arcos.rack/REQUIREMENTS#REQUIREMENT"/>
  </owl:Class>
  <owl:Class rdf:ID="SBVT_Test">
    <rdfs:subClassOf>
      <owl:Restriction>
        <owl:minCardinality rdf:datatype="http://www.w3.org/2001/XMLSchema#int"
        >1</owl:minCardinality>
        <owl:onProperty rdf:resource="http://arcos.rack/TESTING#verifies"/>
      </owl:Restriction>
    </rdfs:subClassOf>
    <rdfs:comment xml:lang="en">A test identified in the Software Baseline Verification Tests</rdfs:comment>
    <rdfs:subClassOf rdf:resource="http://arcos.rack/TESTING#TEST"/>
  </owl:Class>
  <owl:Class rdf:ID="PIDS_Req">
    <rdfs:comment xml:lang="en">A Requirement identified in the Prime Item Development Specification</rdfs:comment>
    <rdfs:subClassOf rdf:resource="http://arcos.rack/REQUIREMENTS#REQUIREMENT"/>
  </owl:Class>
  <owl:Class rdf:ID="CSID_Req">
    <rdfs:comment xml:lang="en">A Requirement identified in the Crew Systems Interface Document</rdfs:comment>
    <rdfs:subClassOf rdf:resource="http://arcos.rack/REQUIREMENTS#REQUIREMENT"/>
  </owl:Class>
  <owl:Class rdf:ID="SBVT_Result">
    <rdfs:subClassOf>
      <owl:Restriction>
        <owl:allValuesFrom rdf:resource="#SBVT_Test"/>
        <owl:onProperty rdf:resource="http://arcos.rack/TESTING#confirms"/>
      </owl:Restriction>
    </rdfs:subClassOf>
    <rdfs:comment xml:lang="en">A result identified for a SBVT_Test (Software Baseline Verification Tests)</rdfs:comment>
    <rdfs:subClassOf rdf:resource="http://arcos.rack/TESTING#TEST_RESULT"/>
  </owl:Class>
</rdf:RDF>
