<rdf:RDF
    xmlns:rdf="http://www.w3.org/1999/02/22-rdf-syntax-ns#"
    xmlns:Arbiter="http://arcos.arbiter/STR#"
    xmlns:builtinfunctions="http://sadl.org/builtinfunctions#"
    xmlns:owl="http://www.w3.org/2002/07/owl#"
    xmlns:sadlimplicitmodel="http://sadl.org/sadlimplicitmodel#"
    xmlns:rdfs="http://www.w3.org/2000/01/rdf-schema#"
    xmlns:sadlbasemodel="http://sadl.org/sadlbasemodel#"
    xmlns:xsd="http://www.w3.org/2001/XMLSchema#"
  xml:base="http://arcos.arbiter/STR">
  <owl:Ontology rdf:about="">
    <owl:imports rdf:resource="http://arcos.rack/MODEL"/>
    <owl:imports rdf:resource="http://arcos.rack/SOFTWARE"/>
    <owl:imports rdf:resource="http://arcos.rack/SYSTEM"/>
    <owl:imports rdf:resource="http://sadl.org/builtinfunctions"/>
    <owl:imports rdf:resource="http://sadl.org/sadlimplicitmodel"/>
    <owl:imports rdf:resource="http://sadl.org/sadlbasemodel"/>
    <rdfs:comment xml:lang="en">This ontology was created from a SADL file 'STR.sadl' and should not be directly edited.</rdfs:comment>
  </owl:Ontology>
  <owl:Class rdf:ID="StrSystem">
    <rdfs:comment xml:lang="en">A component of the logical system with a concept of sequencing dependency</rdfs:comment>
    <rdfs:subClassOf rdf:resource="http://arcos.rack/SYSTEM#SYSTEM"/>
  </owl:Class>
  <owl:Class rdf:ID="StrOutPort">
    <rdfs:comment xml:lang="en">Output interface</rdfs:comment>
    <rdfs:subClassOf rdf:resource="http://arcos.rack/PROV-S#ENTITY"/>
  </owl:Class>
  <owl:Class rdf:ID="StrInPort">
    <rdfs:comment xml:lang="en">Input interface</rdfs:comment>
    <rdfs:subClassOf rdf:resource="http://arcos.rack/PROV-S#ENTITY"/>
  </owl:Class>
  <owl:Class rdf:ID="StrPort">
    <rdfs:subClassOf>
      <owl:Restriction>
        <owl:cardinality rdf:datatype="http://www.w3.org/2001/XMLSchema#int"
        >1</owl:cardinality>
        <owl:onProperty>
          <owl:DatatypeProperty rdf:ID="variableName"/>
        </owl:onProperty>
      </owl:Restriction>
    </rdfs:subClassOf>
    <rdfs:comment xml:lang="en">The communication interface of a concrete software component.</rdfs:comment>
    <rdfs:subClassOf rdf:resource="http://arcos.rack/PROV-S#ENTITY"/>
  </owl:Class>
  <owl:Class rdf:ID="StrEarsModel">
    <rdfs:comment xml:lang="en">A requirement statement written in the Easy Approach to Requirements Syntax language.</rdfs:comment>
    <rdfs:subClassOf rdf:resource="http://arcos.rack/MODEL#MODEL"/>
  </owl:Class>
  <owl:Class rdf:ID="StrComponent">
    <rdfs:comment xml:lang="en">A concrete software component with an explicitly identified input/output interface</rdfs:comment>
    <rdfs:subClassOf rdf:resource="http://arcos.rack/SOFTWARE#SWCOMPONENT"/>
  </owl:Class>
  <owl:ObjectProperty rdf:ID="informs">
    <rdfs:comment xml:lang="en">Informs represents a control or sequencing dependency in the software, with the source of the relationship earlier in the sequence than the target, or alternatively the source activating the target.</rdfs:comment>
    <rdfs:range rdf:resource="#StrSystem"/>
    <rdfs:domain rdf:resource="#StrSystem"/>
  </owl:ObjectProperty>
  <owl:ObjectProperty rdf:ID="recvsVia">
    <rdfs:comment xml:lang="en">Links a component to its incoming interface</rdfs:comment>
    <rdfs:range rdf:resource="#StrInPort"/>
    <rdfs:domain rdf:resource="#StrComponent"/>
  </owl:ObjectProperty>
  <owl:ObjectProperty rdf:ID="sendsVia">
    <rdfs:comment xml:lang="en">Links a component to its outgoing interface</rdfs:comment>
    <rdfs:range rdf:resource="#StrOutPort"/>
    <rdfs:domain rdf:resource="#StrComponent"/>
  </owl:ObjectProperty>
  <owl:ObjectProperty rdf:ID="connectsTo">
    <rdfs:comment xml:lang="en">An association between input and output ports found in the system.</rdfs:comment>
    <rdfs:range rdf:resource="#StrInPort"/>
    <rdfs:domain rdf:resource="#StrOutPort"/>
  </owl:ObjectProperty>
  <owl:DatatypeProperty rdf:about="#variableName">
    <rdfs:comment xml:lang="en">Concrete variable name</rdfs:comment>
    <rdfs:range rdf:resource="http://www.w3.org/2001/XMLSchema#string"/>
    <rdfs:domain rdf:resource="#StrPort"/>
  </owl:DatatypeProperty>
  <owl:DatatypeProperty rdf:ID="earsStatement">
    <rdfs:comment xml:lang="en">Text of statement written in the EARS requirements language.</rdfs:comment>
    <rdfs:range rdf:resource="http://www.w3.org/2001/XMLSchema#string"/>
    <rdfs:domain rdf:resource="#StrEarsModel"/>
  </owl:DatatypeProperty>
  <owl:FunctionalProperty rdf:ID="portType">
    <rdfs:comment xml:lang="en">The type of information communicated over this port</rdfs:comment>
    <rdfs:range rdf:resource="http://www.w3.org/2001/XMLSchema#string"/>
    <rdfs:domain rdf:resource="#StrPort"/>
    <rdf:type rdf:resource="http://www.w3.org/2002/07/owl#DatatypeProperty"/>
  </owl:FunctionalProperty>
</rdf:RDF>
